Declarative/Semantics.v
@@ -1,0 +1,514 @@
+Require Import LanguageUtil.
+Require Import BasicProperties.
+Require Import Properties.
+Require Import Transitivity.
+Require Import Extraction.
+Require Import KindReasoning.
+
+Require Import Program.Tactics.
+
+Definition Progressive (e : expr) : Prop := value e \/ exists e', e ⟶ e'.
+Definition EProgressive (e : eexpr) := evalue e \/ exists e', e ⋆⟶ e'.
+
+Hint Unfold Progressive : core.
+Hint Unfold EProgressive : core.
+
+Ltac instantiate_trivial_equals := repeat
+  match goal with
+  | H : ?a ~= ?a -> _ |- _ => specialize (H JMeq_refl)
+  | H : ?a  = ?a -> _ |- _ => specialize (H eq_refl)
+  end
+.
+
+Hint Extern 1 (lc_expr _) => instantiate_colimits : inst.
+
+Ltac cleanup_hyps := instantiate_trivial_equals; destruct_pairs; clear_dups.
+Ltac solve_progress_value := auto || left; eauto with inst.
+
+Lemma pi_sub_l : forall Γ e A B k,
+    Γ ⊢ e <: e_pi A B : k -> (exists A' B', e = e_pi A' B') \/ (exists C' D', e = e_all C' D').
+Proof.
+  intros.
+  dependent induction H.
+  - eauto.
+  - eauto.
+  - now apply IHusub1 with A B.
+Qed.
+
+Lemma normal_form_forall_pi : forall Γ e A,
+    Γ ⊢ e : A -> value e ->
+    forall C D, A = e_all C D \/ A = e_pi C D ->
+    forall E F k, Γ ⊢ A <: e_pi E F : k ->
+    (exists A' b, e = e_abs A' b) \/ (exists A' b, e = e_bind A' b).
+Proof.
+  intros * H V.
+  dependent induction H.
+    all: try solve [inversion V]. (* solving cases where `e` is not value *)
+    all: intros C' D' [E | E]; inversion E; (* solving invalid cases *)
+      subst; intros; eauto. (* solving trivial base cases *)
+  - assert (G ⊢ A <: e_pi E F : (e_kind k)).
+    now apply transitivity with (e_all C' D') k0.
+    apply pi_sub_l in H3. destruct H3; destruct_exists; subst.
+    eapply IHusub1; eauto.
+    eapply IHusub1; auto.
+    apply transitivity with (e_all C' D') k0; eauto.
+  - assert (G ⊢ A <: e_pi E F : (e_kind k)).
+    now apply transitivity with (e_pi C' D') k0.
+    apply pi_sub_l in H3. destruct H3; destruct_exists; subst.
+    eapply IHusub1; eauto.
+    eapply IHusub1; auto.
+    apply transitivity with (e_pi C' D') k0; eauto.
+Qed.
+
+
+Ltac conclude_type_refl H :=
+  match type of H with
+  | ?G ⊢ _ <: _ : ?A =>
+    let k := fresh "k" in
+    let H := fresh "H" in
+    let contra := fresh "contra" in
+    assert (A = BOX \/ exists k, G ⊢ A : e_kind k) as [contra | [k H]]
+        by (eapply type_correctness; eassumption);
+    try solve [inversion contra]
+  end
+.
+
+Lemma normal_form_pi : forall Γ e A B,
+    Γ ⊢ e : e_pi A B -> value e ->
+    (exists A' b, e = e_abs A' b) \/ (exists A' b, e = e_bind A' b).
+Proof.
+  intros. conclude_type_refl H.
+  eapply normal_form_forall_pi; eauto.
+Qed.
+
+
+Ltac conclude_refls H :=
+  match type of H with
+  | ?G ⊢ ?e1 <: ?e2 : ?A =>
+    let H1 := fresh "H" in
+    let H2 := fresh "H" in
+    assert (H1 : G ⊢ e1 : A) by eauto;
+    assert (H2 : G ⊢ e2 : A) by eauto;
+    conclude_type_refl H
+  end
+.
+
+Ltac invert_to_normal_forms H :=
+  match type of H with
+  | _ ⊢ _ <: _ : e_pi ?A ?B => apply normal_form_pi in H; eauto; destruct H
+  end; destruct_exists; subst
+.
+
+Ltac invert_operator_to_nf :=
+  match goal with
+  | H : _ ⊢ ?e : e_pi _ _ |- ?g =>
+    match g with
+    | context [e] => invert_to_normal_forms H
+    | _ => fail
+    end
+  end
+.
+
+Ltac destruct_progressive_for_app :=
+  let destruct_with_new_name H := (
+      let V := fresh "V" in
+      let e' := fresh "e'" in
+      destruct H as [V | [e' H]])
+  in
+  match goal with
+  | H : Progressive ?e |- exists e', e_app ?e _ ⟶ e' =>
+    destruct_with_new_name H
+  | H : EProgressive ?e |- exists e', ee_app ?e _ ⋆⟶ e' =>
+    destruct_with_new_name H
+  end
+.
+
+Theorem progress : forall e1 e2 A,
+    nil ⊢ e1 <: e2 : A -> Progressive e1 /\ Progressive e2.
+Proof.
+  intros.
+  dependent induction H; cleanup_hyps;
+    try solve [split; solve_progress_value].
+  (* var is not value *)
+  - inversion H0.
+  (* app *)
+  - conclude_refls H0. split; right;
+    destruct_progressive_for_app;
+    eauto 3; (* solves r_app cases *)
+    invert_operator_to_nf.
+    + inversion V; subst. exists (H5 <^^> e). eauto.
+    + inversion V. inversion H11. subst.
+        pick fresh x. instantiate_colimits.
+        exists (e_app (H5 <^> x) e). eauto.
+    + inversion V; subst. exists (H6 <^^> e). eauto.
+    + inversion V; inversion H11. subst.
+        pick fresh x. instantiate_colimits.
+        exists (e_app (H6 <^> x) e). eauto.
+Qed.
+
+Ltac solve_progress_evalue := auto || left; solve_evalue.
+
+Lemma extract_abs : forall A b,
+    ee_abs (extract b) = extract (e_abs A b).
+Proof.
+  easy.
+Qed.
+
+Theorem extracted_progress : forall e1 e2 A,
+    nil ⊢ e1 <: e2 : A -> forall e1' e2', extract e1 = e1' -> extract e2 = e2' ->
+    EProgressive e1' /\ EProgressive e2'.
+Proof.
+  intros * H.
+  dependent induction H; simpl; intros e1' e2' E1 E2; subst; auto;
+    try solve [split; solve_progress_evalue].
+  (* var is not value *)
+  - inversion H0.
+  (* app *)
+  - instantiate_trivial_equals.
+    destruct IHusub2 with (extract e1) (extract e2); auto.
+    conclude_refls H0;
+    split; right; destruct_progressive_for_app; eauto; (* solve r_app cases *)
+      apply evalue_value in V; auto;
+        invert_operator_to_nf; simpl.
+    + exists ((extract H4) ⋆^^ (extract e)). constructor.
+      replace (ee_abs (extract H4)) with (extract (e_abs H2 H4)) by reflexivity.
+      all: eauto using lc_extract_lc.
+    + pick fresh x. exists (ee_app (extract H4 ⋆^ x) (extract e)).
+      eapply er_elim; eauto 3.
+      replace (ee_bind (extract H4)) with (extract (e_bind H2 H4)) by reflexivity.
+      eauto using lc_extract_lc.
+    + exists ((extract H5) ⋆^^ (extract e)). constructor.
+      replace (ee_abs (extract H5)) with (extract (e_abs H3 H5)) by reflexivity.
+      all: eauto using lc_extract_lc.
+    + pick fresh x. exists (ee_app (extract H5 ⋆^ x) (extract e)).
+      eapply er_elim; eauto 3.
+      replace (ee_bind (extract H5)) with (extract (e_bind H3 H5)) by reflexivity.
+      eauto using lc_extract_lc.
+  (* forall_l *)
+  - split.
+    + solve_progress_evalue.
+    + instantiate_trivial_equals.
+      now destruct IHusub3 with (extract (B <^^> e)) (extract C).
+  (* forall_r *)
+  - split.
+    + instantiate_trivial_equals.
+      now destruct IHusub2 with (extract A) (extract A).
+    + solve_progress_evalue.
+Qed.
+
+Ltac find_impossible_reduction :=
+  simpl in *;
+  match goal with
+  | H : ee_app _ _ ⋆⟶ _ |- _ => fail
+  | H : _ ⋆⟶ _ |- _  => solve [inversion H]
+  end
+.
+
+Ltac solve_impossible_reduction := try find_impossible_reduction.
+
+Lemma bind_extraction_inversion : forall e ee,
+    ee_bind ee = extract e ->
+    exists A e', e = e_bind A e' /\ ee = extract e'.
+Proof.
+  induction e; simpl; intros; inversion H; eauto.
+Qed.
+
+Lemma abs_extraction_inversion : forall e ee,
+    ee_abs ee = extract e ->
+    exists A e', e = e_abs A e' /\ ee = extract e'.
+Proof.
+  induction e; simpl; intros; inversion H; eauto.
+Qed.
+
+Ltac invert_extraction :=
+  let A := fresh "A" in
+  let e2 := fresh "e" in
+  let E1 := fresh "E" in
+  let E2 := fresh "E" in
+  match goal with
+  | H : ee_bind ?ee = extract ?e |- _ =>
+    apply bind_extraction_inversion in H as (A & e2 & E1 & E2)
+  | H : ee_abs ?ee = extract ?e |- _ =>
+    apply abs_extraction_inversion in H as (A & e2 & E1 & E2)
+  end; subst; simpl in *
+.
+
+Ltac invert_extractions := repeat invert_extraction.
+
+Lemma abs_not_star : forall Γ A b,
+    not ( Γ ⊢ e_abs A b : * ).
+Proof.
+  intros. intro.
+  dependent induction H.
+  - eapply IHusub1; eauto using star_sub_inversion_l.
+Qed.
+
+Lemma bind_not_star : forall Γ A b,
+    not ( Γ ⊢ e_bind A b : * ).
+Proof.
+  intros. intro.
+  dependent induction H.
+  - eapply IHusub1; eauto using star_sub_inversion_l.
+Qed.
+
+Lemma abs_sub_r : forall Γ A b e T,
+    Γ ⊢ e_abs A b <: e : T ->
+    exists c, e = e_abs A c.
+Proof.
+  intros.
+  dependent induction H.
+  - eauto.
+  - now apply abs_not_star in H0.
+  - now eapply IHusub1.
+Qed.
+
+Lemma abs_sub_l : forall Γ A b e T,
+    Γ ⊢ e <: e_abs A b : T ->
+    exists c, e = e_abs A c.
+Proof.
+  intros.
+  dependent induction H.
+  - eauto.
+  - apply reflexivity_r in H2.
+    now apply abs_not_star in H2.
+  - now eapply IHusub1.
+Qed.
+
+Lemma bind_sub_r : forall Γ A b e T,
+    Γ ⊢ e_bind A b <: e : T ->
+    exists c, e = e_bind A c.
+Proof.
+  intros.
+  dependent induction H.
+  - eauto.
+  - now apply bind_not_star in H0.
+  - now eapply IHusub1.
+Qed.
+
+Lemma bind_sub_l : forall Γ A b e T,
+    Γ ⊢ e <: e_bind A b : T ->
+    exists c, e = e_bind A c.
+Proof.
+  intros. dependent induction H.
+  - eauto.
+  - apply reflexivity_r in H2. now apply bind_not_star in H2.
+  - now eapply IHusub1.
+Qed.
+
+Ltac invert_sub_hyp :=
+  let b := fresh "b" in
+  let E := fresh "E" in
+  let H' := fresh "H" in
+  match goal with
+  | _ : _ ⊢ e_abs _ _  <: e_abs _ _ : _ |- _ => idtac
+  | _ : _ ⊢ e_bind _ _ <: e_bind _ _ : _ |- _ => idtac
+  | H : _ ⊢ e_abs _ _ <: _ : _ |- _ =>
+    pose (H' := H); apply abs_sub_r in H' as (b & E)
+  | H : _ ⊢ _ <: e_abs _ _ : _ |- _ =>
+    pose (H' := H); apply abs_sub_l in H' as (b & E)
+  | H : _ ⊢ e_bind _ _ <: _ : _ |- _ =>
+    pose (H' := H); apply bind_sub_r in H' as (b & E)
+  | H : _ ⊢ _ <: e_bind _ _ : _ |- _ =>
+    pose (H' := H); apply bind_sub_l in H' as (b & E)
+  end; subst; simpl in *
+.
+
+Lemma abs_pi_principal : forall Γ A b1 b2 T,
+    Γ ⊢ e_abs A b1 <: e_abs A b2 : T ->
+    exists B k, Γ ⊢ e_abs A b1 <: e_abs A b2 : e_pi A B /\ Γ ⊢ e_pi A B <: T : e_kind k.
+Proof.
+  intros.
+  dependent induction H.
+  - assert (Sub : G ⊢ e_abs A b1 <: e_abs A b2 : e_pi A B) by eauto.
+    conclude_type_refl Sub. eauto.
+  - edestruct IHusub1 as (B' & k' & Sub & Subpi); eauto.
+    exists B', k'. split.
+    + assumption.
+    + eapply transitivity; eauto.
+Qed.
+
+
+Lemma pi_sub_inversion : forall Γ A B C D k,
+    Γ ⊢ e_pi A B <: e_pi C D : e_kind k ->
+    exists k' L, forall x, x `notin` L ->
+      Γ ⊢ C <: A : e_kind k' /\ Γ, x : C ⊢ B <^> x <: D <^> x : e_kind k.
+Proof.
+  intros.
+  dependent induction H.
+  - exists k1, L. auto.
+  - apply IHusub1; auto.
+    apply kind_sub_inversion_l in H0. destruct_pairs. congruence.
+Qed.
+
+Lemma abs_inversion : forall Γ A b1 b2 T,
+    Γ ⊢ e_abs A b1 <: e_abs A b2 : T ->
+    forall B k,
+    Γ ⊢ T <: e_pi A B : e_kind k ->
+    exists L, forall x, x `notin` L -> Γ, x : A ⊢ b1 <^> x <: b2 <^> x : B <^> x.
+Proof.
+  intros * Sub.
+  dependent induction Sub; intros.
+  - apply pi_sub_inversion in H3 as (k' & L' & H').
+    exists (L `union` L'). intros.
+    instantiate_colimits. destruct_pairs. eauto.
+  - apply IHSub1 with k; eauto using transitivity.
+Qed.
+
+Lemma abs_principal_inversion : forall Γ A b1 b2 B,
+    Γ ⊢ e_abs A b1 <: e_abs A b2 : e_pi A B ->
+    exists L, forall x, x `notin` L -> Γ, x : A ⊢ b1 <^> x <: b2 <^> x : B <^> x.
+Proof.
+  intros.
+  conclude_type_refl H.
+  now apply abs_inversion with (e_pi A B) k.
+Qed.
+
+Lemma bind_inversion : forall Γ A b1 b2 T,
+    Γ ⊢ e_bind A b1 <: e_bind A b2 : T ->
+    exists B L, Γ ⊢ e_bind A b1 <: e_bind A b2 : e_all A B
+         /\ Γ ⊢ e_all A B <: T : *
+         /\ (forall x, x `notin` L -> Γ , x : A ⊢ b1 <^> x <: b2 <^> x : B <^> x)
+         /\ (forall x, x `notin` L -> x `notin` fv_eexpr (extract (b1 <^> x)))
+         /\ (forall x, x `notin` L -> x `notin` fv_eexpr (extract (b2 <^> x))).
+Proof.
+  intros. dependent induction H.
+  - exists B. exists L. repeat split; eauto 2.
+  - specialize (IHusub1 A b1 b2). instantiate_trivial_equals.
+    destruct IHusub1 as (B' & L & IH). destruct_pairs.
+    exists B', L. repeat split; eauto 3 using transitivity.
+Qed.
+
+Definition is_forall (e : expr) : Prop :=
+  match e with
+  | e_all _ _ => True
+  | _ => False
+  end
+.
+
+Lemma forall_l_sub_inversion : forall Γ A B C,
+    Γ ⊢ e_all A B <: C : * ->
+    not (is_forall C) ->
+    exists e, mono_type e /\ Γ ⊢ e : A /\ Γ ⊢ B <^^> e <: C : *.
+Proof.
+  intros * Sub.
+  dependent induction Sub; simpl; intros.
+  + eauto.
+  + contradiction.
+  + contradiction.
+  + eapply IHSub1; eauto.
+    apply kind_sub_inversion_l in Sub2. destruct_pairs. congruence.
+Qed.
+
+Lemma notin_open_var_notin_open_rec : forall e x n,
+    x `notin` fv_eexpr (e ⋆n^^ (ee_var_f x)) ->
+    forall v, e ⋆n^^ v = e.
+Proof.
+  intros e x.
+  induction e; unfold open_eexpr_wrt_eexpr in *; simpl; intros; auto;
+    try solve [rewrite IHe; auto | rewrite IHe1; auto; rewrite IHe2; auto].
+  - destruct (n0 == n).
+    + contradict H. simpl. auto.
+    + easy.
+Qed.
+
+Lemma notin_open_var_notin_open : forall e x v,
+    x `notin` fv_eexpr (e ⋆^ x) ->
+    e ⋆^^ v = e.
+Proof.
+  intros.
+  eapply notin_open_var_notin_open_rec; auto.
+Qed.
+
+Hint Rewrite extract_open_distr : reassoc.
+
+Ltac split_all := repeat split.
+
+Ltac rewrite_open_with_subst_impl G :=
+  match G with
+  | context [?e <^^> ?v] =>
+    progress
+      match v with
+      | e_var_f _ => idtac
+      | _ => erewrite (open_subst_eq e); eauto
+      end
+  end
+.
+
+Ltac rewrite_open_with_subst :=
+  repeat
+    match goal with
+    | |- ?g => rewrite_open_with_subst_impl g
+    end
+.
+
+Ltac rewrite_extract_invariant G e :=
+  match G with
+  | context [e ⋆^^ _] =>
+    erewrite (notin_open_var_notin_open e); eauto
+  end
+.
+
+Ltac find_extract_invariants :=
+  repeat
+    match goal with
+    | H : ?x `notin` fv_eexpr (extract _) |- _  => autorewrite with reassoc in H; simpl in H
+    | H : ?x `notin` fv_eexpr (?e ⋆^ ?x) |- ?G => rewrite_extract_invariant G e
+    | _ => progress autorewrite with reassoc
+    end
+.
+
+Theorem preservation : forall e1 e2 A,
+    nil ⊢ e1 <: e2 : A ->
+    forall e1'' e2'', extract e1 ⋆⟶ e1'' -> extract e2 ⋆⟶ e2''  ->
+    exists e1' e2', extract e1' = e1''
+             /\ extract e2' = e2''
+             /\ e1 ⟶ e1'
+             /\ e2 ⟶ e2'
+             /\ nil ⊢ e1' <: e2' : A.
+Proof.
+  intros * Sub.
+  dependent induction Sub; simpl; intros;
+    solve_impossible_reduction;
+    instantiate_trivial_equals.
+  - inversion H0; subst.
+    + inversion H1; subst.
+      (* main case for r_app *)
+      * destruct IHSub2 with ee2 ee0 as (e1' & e2' & IH); eauto.
+        destruct_conjs. subst.
+        exists (e_app e1' e), (e_app e2' e). repeat split; eauto 3.
+      * invert_extractions. invert_sub_hyp. solve_impossible_reduction.
+      * invert_extractions. invert_sub_hyp. solve_impossible_reduction.
+    + invert_extractions. invert_sub_hyp.
+      inversion H1; subst; solve_impossible_reduction.
+      (* main case for r_beta *)
+      exists (e0 <^^> e), (b <^^> e).
+      autorewrite with reassoc.
+      split_all; eauto.
+      pose (B' := Sub2). apply abs_pi_principal in B'. destruct_conjs.
+      apply pi_sub_inversion in H7 as (k' & L & Sub3).
+      apply abs_principal_inversion in H3 as (L' & Sub4).
+      pick fresh x for
+           (L `union` L' `union` fv_expr e0 `union` fv_expr b `union` fv_expr B).
+      instantiate_colimits. destruct_pairs.
+      rewrite_open_with_subst.
+      eauto 4 using substitution_cons, ctx_narrowing_cons.
+    + invert_extractions. invert_sub_hyp.
+      inversion H1; subst; solve_impossible_reduction.
+      (* main case for r_inst *)
+      apply bind_inversion in Sub2 as (F & L1 & Hb). destruct_pairs.
+      apply forall_l_sub_inversion in H3 as (m & M & Subm & Sub_inst); auto.
+      exists (e_app (e0 <^^> m) e), (e_app (b <^^> m) e). split_all; simpl.
+      * pick fresh x'. instantiate_colimits. find_extract_invariants.
+      * pick fresh x'. instantiate_colimits. find_extract_invariants.
+      * eauto.
+      * eauto.
+      * eapply s_app; eauto. apply s_sub with (F <^^> m) k_star; auto.
+        pick fresh x' for
+             (L `union` L0 `union` L1 `union`
+                fv_expr e0 `union` fv_expr b `union` fv_expr F).
+        rewrite_open_with_subst.
+        eauto 3 using substitution_cons.
+  - edestruct IHSub1 as (e1' & e2' & H1); eauto.
+    destruct_pairs.
+    exists e1', e2'. repeat split; eauto.
+Qed.
